\begin{align*}
& \text{We denote the generalized term,} \ [k] \ \text{as}\ldots \\
& [k]: \ 2^k T(n/2^k) + \sum_{i=0}^{k-1} 2^i \log_2 (n/2^i) \\
& \text{At some point: } \ T(n/2^k) = 1, \ \text{i.e.} \ n/2^k = 1. \\
& n/2^k = 1 \equiv n/2^{\log_2 n} \ \therefore k = \log_2 n \\
& \text{Substitute } \ \log_2 n \ \text{for } \ k \ \text{in} \ [k]: \
{2^{\log_2 n}}(1) + \sum_{i=0}^{(\log_2 n)-1} 2^i \log_2 (n/2^i) \\
& \text{Solving the left operand}: 2^{\log_2 n} \Leftrightarrow \log_2 2^n = n \times \log_2 2 = n \times 1 = n \\
& \text{Updating } \ [k]: n + \sum_{i=0}^{(\log_2 n)-1} 2^i \log_2 (n/2^i) \\
\end{align*}